automation/super/clause_ops.lean
@@ -21,10 +21,11 @@ qf : clause × list expr ← ↑(c↣open_constn c↣num_quants),
 op : clause × list expr ← ↑(qf↣1↣open_constn c↣num_lits),
 lci ← (op↣2↣nth i)↣to_monad,
 () : unit ← ↑(@guard tactic _ ((qf↣1↣get_lit i)↣is_neg) _),
-h ← ↑(mk_local_def `h (qf↣1↣get_lit i)↣formula↣not_),
+h ← ↑(mk_local_def `h (imp (qf↣1↣get_lit i)↣formula c↣local_false)),
 new_hyps ← f h,
 return $ new_hyps↣for $ λnew_hyp,
-  (((clause.mk 0 0 new_hyp↣2 false_)↣close_const h)↣inst (op↣1↣close_const lci)↣proof)↣close_constn
+  (((clause.mk 0 0 new_hyp↣2 c↣local_false c↣local_false)↣close_const h)↣inst
+               (op↣1↣close_const lci)↣proof)↣close_constn
   (qf↣2 ++ op↣2↣remove i ++ new_hyp↣1)
 
 meta def on_right_at {m} [monad m] (c : clause) (i : ℕ)
@@ -48,8 +49,7 @@ h ← ↑(mk_local_def `h (op↣1↣get_lit 0)↣formula),
 new_hyps ← f h,
 forM new_hyps (λnew_hyp, do
   type ← ↑(infer_type new_hyp↣2),
-  nhn ← ↑mk_fresh_name,
-  nh ← return $ local_const nhn `nh binder_info.default (imp type false_),
+  nh ← ↑(mk_local_def `nh (imp type c↣local_false)),
   return $ (op↣1↣inst (lambdas [h] (app nh new_hyp↣2)))↣close_constn (op↣2 ++ new_hyp↣1 ++ [nh]))
 
 meta def on_first_right (c : clause) (f : expr → tactic (list (list expr × expr))) : tactic (list clause) :=
