automation/super/prover.lean
@@ -84,11 +84,14 @@ open super
 
 meta def super (sos_lemmas : list expr) : tactic unit := do
 intros,
-target_name ← get_unused_name `target none, tgt ← target,
-mk_mapp ``classical.by_contradiction [some tgt] >>= apply, intro target_name,
+local_false_name ← get_unused_name `F none, tgt ← target, tgt_type ← infer_type tgt,
+definev local_false_name tgt_type tgt, local_false ← get_local `F,
+target_name ← get_unused_name `target none,
+assertv target_name (imp tgt local_false) (lam `hf binder_info.default tgt $ mk_var 0),
+change local_false,
 hyps ← local_context,
-initial_clauses ← mapM clause.of_proof (hyps ++ sos_lemmas),
-initial_state ← resolution_prover_state.initial initial_clauses,
+initial_clauses ← mapM (clause.of_proof local_false) (hyps ++ sos_lemmas),
+initial_state ← resolution_prover_state.initial local_false initial_clauses,
 res ← run_prover_loop selection21 (age_weight_clause_selection 6 7)
   default_preprocessing default_inferences
   0 initial_state,
